\documentclass[main.tex]{subfiles}

\begin{document}
\sloppy


\vspace{1.0cm}

\begin{equation}
\begin{aligned}

\text{if(stavamo accelerando)\{} \\
2x + 2 = 4\\
\text{\}}

\end{aligned}
\end{equation}

\newline

$\text{stopDistanceWhenWeReach1} = \text{movementUpTo1} + \text{stopDistance}$
$stopDistanceWhenWeReach1 = distanceUpTo1 + stopDistance$
\newline

\[T =%
	%\begin{dcases}%
		T = \frac{D}{S_i} & \text{se } S_i = S_{i - 1}\\
		\hfil \frac{a}{4}x^2 - S_ix + D & \text{altrimenti}
	%\end{dcases}%
\]

\[t = \frac{D_i}{S_i} \qquad \text{se } S_i = S_{i - 1}\]
\[\frac{a}{4}t^2 - S_it + D_i = 0 \quad \text{altrimenti}\]

\newline

\[t = s - \frac{2D}{S_{i - 1}}\]
\[a = \frac{0 - S_{i - 1}}{t - 0} = - \frac{S_{i - 1}}{t}\]

\[\frac{S_i\abs{Tx - TS_i}}{2} + \frac{x\abs{Tx - TS_i}}{2} + \frac{Tx^2}{2} + tx - D = 0\]

\newline

\[y > \tan(R)x + (A - \frac{\tan(R)}{2})\]
\[y > x(B - A) + A\]

\[i > \sqrt{(2x - 1)^2 + (2y - 1)^2}\]

\[d = \abs{y - g(x)}\]
\[d = \abs{\sqrt{(2x - 1)^2 + (2y - 1)^2} - i}\]

\[\text{Se} \quad A_t < D\]
\[\text{Se} \quad A_t \geq D\]

\[m_i = m_{i - 1} - (1 - f_i)\]

\end{document}